Substantially overhauled the implementation of local variables. This is now done by an explicit injection universe and we don't use polymorphic UTP theories as the current overloading primitives limit what we can do with these at the type level. Nevertheless, the infrastructure is generic and can be applied to a number of UTP theories. Automation is also much improved.

utp/utp_local.thy
@@ -1,144 +1,206 @@
-subsection {* Variable blocks *}
+subsection {* Local Variables *}
 
 theory utp_local
-imports utp_theory
+imports 
+  utp_rel_laws 
+  utp_meta_subst 
+  utp_theory
 begin
+      
+subsection {* Preliminaries *}
+  
+text {* The following type is used to augment that state-space with a stack of local variables
+  represented as a list in the special variable $store$. Local variables will be represented
+  by pushing variables onto the stack, and popping them off after use. The element type of
+  the stack is @{typ "'u"} which corresponds to a suitable injection universe. *}
+  
+alphabet 'u local =
+  store :: "'u list"
 
-text {* Local variables are represented as lenses whose view type is a list of values. A variable
-  therefore effectively records the stack of values that variable has had, if any. This allows
-  us to denote variable scopes using assignments that push and pop this stack to add or delete
-  a particular local variable. *}
-
-type_synonym ('a, '\<alpha>) lvar = "('a list \<Longrightarrow> '\<alpha>)"
-
-text {* Next, we define constants to represent the top most variable on the local variable stack,
-  and the remainder after this. We define these in terms of the list lens, and so for each
-  another lens is produced. *}
-
-definition top_var :: "('a::two, '\<alpha>) lvar \<Rightarrow> ('a \<Longrightarrow> '\<alpha>)" where
-[upred_defs]: "top_var x = (list_lens 0 ;\<^sub>L x)"
-
-text {* The remainder of the local variable stack (the tail) *}
-
-definition rest_var :: "('a::two, '\<alpha>) lvar \<Rightarrow> ('a list \<Longrightarrow> '\<alpha>)" where
-[upred_defs]: "rest_var x = (tl_lens ;\<^sub>L x)"
-
-text {* We can show that the top variable is a mainly well-behaved lense, and that the top most
-  variable lens is independent of the rest of the stack. *}
-
-lemma top_mwb_lens [simp]: "mwb_lens x \<Longrightarrow> mwb_lens (top_var x)"
-  by (simp add: list_mwb_lens top_var_def)
-
-lemma top_rest_var_indep [simp]:
-  "mwb_lens x \<Longrightarrow> top_var x \<bowtie> rest_var x"
-  by (simp add: lens_indep_left_comp rest_var_def top_var_def)
-
-lemma top_var_pres_indep [simp]:
-  "x \<bowtie> y \<Longrightarrow> top_var x \<bowtie> y"
-  by (simp add: lens_indep_left_ext top_var_def)
-
-syntax
-  "_top_var"             :: "svid \<Rightarrow> svid" ("@_" [999] 999)
-  "_rest_var"            :: "svid \<Rightarrow> svid" ("\<down>_" [999] 999)
-
-translations
-  "_top_var x" == "CONST top_var x"
-  "_rest_var x" == "CONST rest_var x"
-
-text {* With operators to represent local variables, assignments, and stack manipulation defined,
-  we can go about defining variable blocks themselves. *}
-
-definition var_begin :: "('\<T>, '\<alpha>) uthy \<Rightarrow> ('a, '\<beta>) lvar \<Rightarrow> '\<alpha> hrel" where
-[urel_defs]: "var_begin T x = x ::=\<^bsub>T\<^esub> \<langle>\<guillemotleft>undefined\<guillemotright>\<rangle> ^\<^sub>u &x"
-
-definition var_end :: "('\<T>, '\<alpha>) uthy \<Rightarrow> ('a, '\<beta>) lvar \<Rightarrow> '\<alpha> hrel" where
-[urel_defs]: "var_end T x = (x ::=\<^bsub>T\<^esub> tail\<^sub>u(&x))"
-
-text {* @{const var_begin} takes as parameters a UTP theory and a local variable, and uses the
-  theory assignment operator to push and undefined value onto the variable stack. @{const var_end}
-  removes the top most variable from the stack in a similar way. *}
-
-definition var_vlet :: "('\<T>, '\<alpha>) uthy \<Rightarrow> ('a, '\<alpha>) lvar \<Rightarrow> '\<alpha> hrel" where
-[urel_defs]: "var_vlet T x = (($x \<noteq>\<^sub>u \<langle>\<rangle>) \<and> \<I>\<I>\<^bsub>T\<^esub>)"
-
-text {* Next we set up the typical UTP variable block syntax, though with a suitable subscript index
-  to represent the UTP theory parameter. *}
-
-syntax
-  "_var_begin"     :: "logic \<Rightarrow> svid \<Rightarrow> logic" ("var\<index> _" [100] 100)
-  "_var_begin_asn" :: "logic \<Rightarrow> svid \<Rightarrow> logic \<Rightarrow> logic" ("var\<index> _ := _")
-  "_var_end"       :: "logic \<Rightarrow> svid \<Rightarrow> logic" ("end\<index> _" [100] 100)
-  "_var_vlet"      :: "logic \<Rightarrow> svid \<Rightarrow> logic" ("vlet\<index> _" [100] 100)
-  "_var_scope"           :: "logic \<Rightarrow> svid \<Rightarrow> logic \<Rightarrow> logic" ("var\<index> _ \<bullet> _" [0,10] 10)
-  "_var_scope_ty"        :: "logic \<Rightarrow> svid \<Rightarrow> type \<Rightarrow> logic \<Rightarrow> logic" ("var\<index> _ :: _ \<bullet> _" [0,0,10] 10)
-  "_var_scope_ty_assign" :: "logic \<Rightarrow> svid \<Rightarrow> type \<Rightarrow> logic \<Rightarrow> logic \<Rightarrow> logic" ("var\<index> _ :: _ := _ \<bullet> _" [0,0,0,10] 10)
-
-translations
-  "_var_begin T x"       == "CONST var_begin T x"
-  "_var_begin_asn T x e" => "var\<^bsub>T\<^esub> x ;; @x ::=\<^bsub>T\<^esub> e"
-  "_var_end T x"         == "CONST var_end T x"
-  "_var_vlet T x"        == "CONST var_vlet T x"
-  "var\<^bsub>T\<^esub> x \<bullet> P" => "var\<^bsub>T\<^esub> x ;; ((\<lambda> x. P) (CONST top_var x)) ;; end\<^bsub>T\<^esub> x"
-  "var\<^bsub>T\<^esub> x \<bullet> P" => "var\<^bsub>T\<^esub> x ;; ((\<lambda> x. P) (CONST top_var x)) ;; end\<^bsub>T\<^esub> x"
-
-text {* In order to substantiate standard variable block laws, we need some underlying laws about
-  assignments, which is the purpose of the following locales. *}
-
-locale utp_prog_var = utp_theory \<T> for \<T> :: "('\<T>, '\<alpha>) uthy" (structure) +
-  fixes \<V>\<T> :: "'\<beta> itself"
-  assumes pvar_uvar: "vwb_lens (\<^bold>s :: '\<beta> \<Longrightarrow> '\<alpha>)"
-  and Healthy_pvar_assigns [closure]: "\<^bold>\<langle>\<sigma> :: '\<beta> usubst\<^bold>\<rangle> is \<H>"
-  and pvar_assigns_comp: "(\<^bold>\<langle>\<sigma>\<^bold>\<rangle> ;; \<^bold>\<langle>\<rho>\<^bold>\<rangle>) = \<^bold>\<langle>\<rho> \<circ> \<sigma>\<^bold>\<rangle>"
-
-text {* We require that (1) the user-space variable is a very well-behaved lens, (2) that the
-  assignment operator is healthy, and (3) that composing two assignments is equivalent to
-  composing their substitutions. The next locale extends this with a left unit. *}
-
-locale utp_local_var = utp_prog_var \<T> V + utp_theory_left_unital \<T> for \<T> :: "('\<T>, '\<alpha>) uthy" (structure) and V :: "'\<beta> itself" +
-  assumes pvar_assign_unit: "\<^bold>\<langle>id :: '\<beta> usubst\<^bold>\<rangle> = \<I>\<I>"
-begin
-
-text {* If a left unit exists then an assignment with an identity substitution should yield the
-  identity relation, as the above assumption requires. With these laws available, we can
-  prove the main laws of variable blocks. *}
-
-lemma var_begin_healthy [closure]:
-  fixes x :: "('a, '\<beta>) lvar"
-  shows "var x is \<H>"
-  by (simp add: var_begin_def Healthy_pvar_assigns)
-
-lemma var_end_healthy [closure]:
-  fixes x :: "('a, '\<beta>) lvar"
-  shows "end x is \<H>"
-  by (simp add: var_end_def Healthy_pvar_assigns)
-
-text {* The beginning and end of a variable block are both healthy theory elements. *}
-
-lemma var_open_close:
-  fixes x :: "('a, '\<beta>) lvar"
-  assumes "vwb_lens x"
-  shows "(var x ;; end x) = \<I>\<I>"
-  by (simp add: var_begin_def var_end_def shEx_lift_seq_1 Healthy_pvar_assigns pvar_assigns_comp pvar_assign_unit usubst assms)
-
-text {* Opening and then immediately closing a variable blocks yields a skip. *}
+text {* The following predicate wraps the relation with assumptions that the stack has a particular 
+  size before and after execution. *}
+  
+definition local_num where
+"local_num n P = [#\<^sub>u(&store) =\<^sub>u \<guillemotleft>n\<guillemotright>]\<^sup>\<top> ;; P ;; [#\<^sub>u(&store) =\<^sub>u \<guillemotleft>n\<guillemotright>]\<^sup>\<top>"
+  
+declare inj_univ.from_univ_def [upred_defs]
+declare inj_univ.to_univ_lens_def [upred_defs]
+declare nat_inj_univ_def [upred_defs]
     
-lemma var_open_close_commute:
-  fixes x :: "('a, '\<beta>) lvar" and y :: "('b, '\<beta>) lvar"
-  assumes "vwb_lens x" "vwb_lens y" "x \<bowtie> y"
-  shows "(var x ;; end y) = (end y ;; var x)"
-  by (simp add: var_begin_def var_end_def shEx_lift_seq_1 shEx_lift_seq_2
-                Healthy_pvar_assigns pvar_assigns_comp
-                assms usubst unrest  lens_indep_sym, simp add: assms usubst_upd_comm)
+subsection {* State Primitives *}
+  
+text {* The following record is used to characterise the UTP theory specific operators we require
+  in order to create the local variable operators. *}
+  
+record ('\<alpha>, 's) state_prim =
+  
+  -- {* The first field states where in the alphabet @{typ "'\<alpha>"} the user state-space type is 
+        @{typ "'s"} is located with the form of a lens. *}
 
-text {* The beginning and end of variable blocks from different variables commute. *}
+  sstate   :: "'s \<Longrightarrow> '\<alpha>" ("\<^bold>s\<index>") 
 
-lemma var_block_vacuous:
-  fixes x :: "('a::two, '\<beta>) lvar"
-  assumes "vwb_lens x"
-  shows "(var x \<bullet> \<I>\<I>) = \<I>\<I>"
-  by (simp add: Left_Unit assms var_end_healthy var_open_close)
+  -- {* The second field is the theory's substitution operator. It takes a substitution over the
+        state-space type and constructs a homogeneous assignment relation. *}
 
-text {* A variable block with a skip inside results in a skip. *}
+  sassigns :: "'s usubst \<Rightarrow> '\<alpha> hrel" ("\<^bold>\<langle>_\<^bold>\<rangle>\<index>")
+  
+syntax
+  "_sstate" :: "logic \<Rightarrow> svid" ("\<^bold>s\<index>")
+
+translations
+  "_sstate T" => "CONST sstate T"
+
+text {* The following record type adds an injection universe @{typ "'u"} to the above operators.
+  This is needed because the stack has a homogeneous type into which we must inject type variable
+  bindings. The universe can be any Isabelle type, but must satisfy the axioms of the locale
+  @{term inj_univ}, which broadly shows the injectable values permitted. *}
+  
+record ('\<alpha>, 's, 'u, 'a) local_prim = "('\<alpha>, ('u, 's) local_scheme) state_prim" +
+  inj_local :: "('a, 'u) inj_univ"
+  
+text {* The following locales give the assumptions required of the above signature types. The first
+  gives the definining axioms for state-spaces. State-space lens @{text "\<^bold>s"} must be a very well-behaved
+  lens, and sequential composition of assignments corresponds to functional composition of the
+  underlying substitutions. TODO: We might also need operators to properly handle framing in the
+  future. *}
+  
+locale utp_state =
+  fixes S (structure)
+  assumes "vwb_lens \<^bold>s"
+  and passigns_comp: "(\<^bold>\<langle>\<sigma>\<^bold>\<rangle> ;; \<^bold>\<langle>\<rho>\<^bold>\<rangle>) = \<^bold>\<langle>\<rho> \<circ> \<sigma>\<^bold>\<rangle>"
+      
+text {* The next locale combines the axioms of a state-space and an injection universe structure. It
+  then uses the required constructs to create the local variable operators. *}
+  
+locale utp_local_state = utp_state S + inj_univ "inj_local S" for S :: "('\<alpha>, 's, 'u::two, 'a) local_prim" (structure)
+begin
+
+  text {* The following two operators represent opening and closing a variable scope, which is
+   implemented by pushing an arbitrary initial value onto the stack, and popping it off, respectively. *}
+  
+  definition var_open :: "'\<alpha> hrel" ("open\<^sub>v") where
+  "var_open = (\<Sqinter> v \<bullet> \<^bold>\<langle>[store \<mapsto>\<^sub>s (&store ^\<^sub>u \<langle>\<guillemotleft>v\<guillemotright>\<rangle>)]\<^bold>\<rangle>)"
+  
+  definition var_close :: "'\<alpha> hrel" ("close\<^sub>v") where
+  "var_close = \<^bold>\<langle>[store \<mapsto>\<^sub>s front\<^sub>u(&store) \<triangleleft> #\<^sub>u(&store) >\<^sub>u 0 \<triangleright> &store]\<^bold>\<rangle>"
+  
+  text {* The next operator is an expression that returns a lens pointing to the top of the stack.
+    This is effectively a dynamic lens, since where it points to depends on the initial number
+    of variables on the stack. *}
+  
+  definition top_var :: "('a \<Longrightarrow> ('u, 'b) local_scheme, '\<alpha> \<times> '\<alpha>) uexpr" ("top\<^sub>v") where
+  "top_var = \<guillemotleft>\<lambda> l. to_univ_lens ;\<^sub>L list_lens l ;\<^sub>L store\<guillemotright>(#\<^sub>u($\<^bold>s:store) - 1)\<^sub>a"
+  
+  text {* Finally, we combine the above operators to represent variable scope. This is a kind of
+    binder which takes a homogeneous relation, parametric over a lens, and returns a relation. It
+    simply opens the variable scope, substitutes the top variable into the body, and then closes
+    the scope afterwards. *}
+  
+  definition var_scope :: "(('a \<Longrightarrow> ('u, 's) local_scheme) \<Rightarrow> '\<alpha> hrel) \<Rightarrow> '\<alpha> hrel" where
+  "var_scope f = open\<^sub>v ;; f(x)\<lbrakk>x\<rightarrow>top\<^sub>v\<rbrakk> ;; close\<^sub>v" 
 end
+
+notation utp_local_state.var_open ("open[_]")
+notation utp_local_state.var_close ("close[_]")  
+  
+syntax       
+  "_var_scope"      :: "logic \<Rightarrow> id \<Rightarrow> logic \<Rightarrow> logic" ("var[_] _ \<bullet> _" [0, 0, 10] 10)
+  "_var_scope_type" :: "logic \<Rightarrow> id \<Rightarrow> type \<Rightarrow> logic \<Rightarrow> logic" ("var[_] _ :: _ \<bullet> _" [0, 0, 0, 10] 10)
+
+translations
+  "_var_scope T x P" == "CONST utp_local_state.var_scope T (\<lambda> x. P)"
+  "_var_scope_type T x t P" => "CONST utp_local_state.var_scope T (_abs (_constrain x (_uvar_ty t)) P)"
+    
+text {* Next, we prove a collection of important generci laws about variable scopes using the axioms
+  defined above. *}
+  
+context utp_local_state
+begin
+  
+  lemma var_open_commute:
+    "\<lbrakk> x \<bowtie> store; store \<sharp> v \<rbrakk> \<Longrightarrow> \<^bold>\<langle>[x \<mapsto>\<^sub>s v]\<^bold>\<rangle> ;; open\<^sub>v = open\<^sub>v ;; \<^bold>\<langle>[x \<mapsto>\<^sub>s v]\<^bold>\<rangle>"
+    by (simp add: var_open_def passigns_comp seq_UINF_distl' seq_UINF_distr' usubst unrest lens_indep_sym, simp add: usubst_upd_comm)
+
+  lemma var_close_commute:
+    "\<lbrakk> x \<bowtie> store; store \<sharp> v \<rbrakk> \<Longrightarrow> \<^bold>\<langle>[x \<mapsto>\<^sub>s v]\<^bold>\<rangle> ;; close\<^sub>v = close\<^sub>v ;; \<^bold>\<langle>[x \<mapsto>\<^sub>s v]\<^bold>\<rangle>"
+    by (simp add: var_close_def passigns_comp seq_UINF_distl' seq_UINF_distr' usubst unrest lens_indep_sym, simp add: usubst_upd_comm)
+
+  lemma var_open_close_lemma: 
+    "[store \<mapsto>\<^sub>s front\<^sub>u(&store ^\<^sub>u \<langle>\<guillemotleft>v\<guillemotright>\<rangle>) \<triangleleft> 0 <\<^sub>u #\<^sub>u(&store ^\<^sub>u \<langle>\<guillemotleft>v\<guillemotright>\<rangle>) \<triangleright> &store ^\<^sub>u \<langle>\<guillemotleft>v\<guillemotright>\<rangle>] = id"
+    by (rel_auto)
+  
+  lemma var_open_close: "open\<^sub>v ;; close\<^sub>v = \<^bold>\<langle>id\<^bold>\<rangle>"
+    by (simp add: var_open_def var_close_def seq_UINF_distr' passigns_comp usubst var_open_close_lemma)
+      
+  lemma var_scope_skip: "(var[S] x \<bullet> \<^bold>\<langle>id\<^bold>\<rangle>) = \<^bold>\<langle>id\<^bold>\<rangle>"
+    by (simp add: var_scope_def var_open_def var_close_def seq_UINF_distr' passigns_comp var_open_close_lemma usubst)  
+
+  (* A property we'd like to prove globally, but requires additional laws for assignment that may
+     not be possible generically. *)
+      
+  lemma var_scope_nonlocal_left: 
+    "\<lbrakk> x \<bowtie> store ; store \<sharp> v \<rbrakk> \<Longrightarrow> \<^bold>\<langle>[x \<mapsto>\<^sub>s v]\<^bold>\<rangle> ;; (var[S] y \<bullet> P(y)) = (var[S] y \<bullet> \<^bold>\<langle>[x \<mapsto>\<^sub>s v]\<^bold>\<rangle> ;; P(y))"
+  oops
+      
+end
+                   
+declare utp_local_state.var_open_def [upred_defs]
+declare utp_local_state.var_close_def [upred_defs]  
+declare utp_local_state.top_var_def [upred_defs]
+declare utp_local_state.var_scope_def [upred_defs]  
+  
+subsection {* Relational State Spaces *}
+  
+text {* To illustrate the above technique, we instantiate it for relations with a @{typ nat} as
+  the universe type. The following definition defines the state-space location, assignment operator,
+  and injection universe for this. *}
+  
+definition rel_local_state :: 
+  "'a::countable itself \<Rightarrow> ((nat, 's) local_scheme, 's, nat, 'a::countable) local_prim" where
+  "rel_local_state t = \<lparr> sstate = 1\<^sub>L, sassigns = assigns_r, inj_local = nat_inj_univ \<rparr>"
+  
+abbreviation rel_local ("R\<^sub>l") where
+"rel_local \<equiv> rel_local_state TYPE('a::countable)"
+  
+syntax
+  "_rel_local_state_type" :: "type \<Rightarrow> logic" ("R\<^sub>l[_]")
+  
+translations
+  "_rel_local_state_type a" => "CONST rel_local_state (_TYPE a)"
+  
+lemma get_rel_local [lens_defs]:
+  "get\<^bsub>\<^bold>s\<^bsub>R\<^sub>l\<^esub>\<^esub> = id"
+  by (simp add: rel_local_state_def lens_defs)
+  
+lemma rel_local_state [simp]: "utp_local_state R\<^sub>l"
+  by (unfold_locales, simp_all add: upred_defs assigns_comp rel_local_state_def)
+
+lemma sassigns_rel_state [simp]: "\<^bold>\<langle>\<sigma>\<^bold>\<rangle>\<^bsub>R\<^sub>l\<^esub> = \<langle>\<sigma>\<rangle>\<^sub>a"
+  by (simp add: rel_local_state_def)
+
+syntax
+  "_rel_var_scope"      :: "id \<Rightarrow> logic \<Rightarrow> logic" ("var _ \<bullet> _" [0, 10] 10)
+  "_rel_var_scope_type" :: "id \<Rightarrow> type \<Rightarrow> logic \<Rightarrow> logic" ("var _ :: _ \<bullet> _" [0, 0, 10] 10)
+
+translations
+  "_rel_var_scope x P" => "_var_scope R\<^sub>l x P"
+  "_rel_var_scope_type x t P" => "_var_scope_type (_rel_local_state_type t) x t P"
+ 
+text {* Next we prove some examples laws. *}
+  
+lemma rel_var_ex_1: "(var x :: string \<bullet> II) = II"
+  by (rel_auto')
+
+lemma rel_var_ex_2: "(var x \<bullet> x := 1) = II"
+  by (rel_auto')
+   
+lemma rel_var_ex_3: "x \<bowtie> store \<Longrightarrow> x := 1 ;; open[R\<^sub>l['a::countable]] = open[R\<^sub>l['a]] ;; x := 1"
+  by (metis pr_var_def rel_local_state sassigns_rel_state unrest_one utp_local_state.var_open_commute)
+
+lemma rel_var_ex_4: "\<lbrakk> x \<bowtie> store; store \<sharp> v \<rbrakk> \<Longrightarrow> x := v ;; open[R\<^sub>l['a::countable]] = open[R\<^sub>l['a]] ;; x := v"
+  by (metis pr_var_def rel_local_state sassigns_rel_state utp_local_state.var_open_commute)
+ 
+lemma rel_var_ex_5: "\<lbrakk> x \<bowtie> store; store \<sharp> v \<rbrakk> \<Longrightarrow> x := v ;; (var y :: int \<bullet> P) = (var y :: int \<bullet> x := v ;; P)"
+  by (simp add: utp_local_state.var_scope_def seqr_assoc[THEN sym] rel_var_ex_4, rel_auto', force+)
 
 end
